coq:set theory

coq/set/Lang1/Specification.v
@@ -13,26 +13,26 @@ Require Import Lang1.Semantics.
 Require Import Lang1.Relevance.
 Require Import Lang1.Environment.
 
-(* Theorem schema 'comprehensionLEM' expressed in set theory abstract syntax.   *)
+(* Theorem schema 'specificationLEM' expressed in set theory abstract syntax.   *)
 (* The formulation is parameterized with respect to a formula P, hence this is  *)
 (* not a single theorem, but rather a 'theorem schema'. This formulation is     *)
 (* correct provided the variables n m p are distinct and m is not free in P.    *)
-Definition comprehensionF (P : Formula) (n m p:nat) : Formula :=
+Definition specificationF (P : Formula) (n m p:nat) : Formula :=
     All n (Exi m (All p (Iff (Elem p m) (And (Elem p n) P)))). 
 
-(* Evaluating comprehensionF applied to a formula P in any environment 'yields' *)
-(* the theorem comprehensionLEM applied to the corresponding predicate.         *)
-Lemma evalComprehensionF : LEM -> forall (e:Env) (P: Formula) (n m p:nat),
+(* Evaluating specificationF applied to a formula P in any environment 'yields' *)
+(* the theorem specificationLEM applied to the corresponding predicate.         *)
+Lemma evalSpecificationF : LEM -> forall (e:Env) (P: Formula) (n m p:nat),
     m <> n ->
     p <> n ->
     p <> m ->
     ~In m (free P) ->
-    eval e (comprehensionF P n m p)
+    eval e (specificationF P n m p)
         <->
     forall (x:set), exists (y:set), forall (z:set),
         z :: y <-> z :: x /\ (eval2 e P n p x z).
 Proof.
-    intros L e P n m p Hmn Hpn Hpm NF. unfold comprehensionF. rewrite evalAll.
+    intros L e P n m p Hmn Hpn Hpm NF. unfold specificationF. rewrite evalAll.
     split; intros H x. 
     - remember (H x) as H' eqn:E. clear E H. rewrite evalExi in H'.
       destruct H' as [y H]. exists y. rewrite evalAll in H. intros z.
